src/dafny/utils/NativeTypes.dfy
@@ -47,4 +47,15 @@ module NativeTypes {
     newtype{:nativeType "int"} nat32 = i:int | 0 <= i < 0x80000000
     newtype{:nativeType "long"} nat64 = i:int | 0 <= i < 0x8000000000000000
 
+    /**
+     * Bitwise exclusive-or of two `uint8` value
+     *
+     * @param a  First value
+     * @param b  Second value
+     * @returns  Bitwise exclusive-or of `a` and `b`
+     */
+    function uint8xor(a:uint8, b:uint8): uint8
+    {
+        ((a as bv8)^(b as bv8)) as uint8
+    }    
 } 
